theories/simplang/gen_refl.v
@@ -1,131 +1,13 @@
 From simuliris.simulation Require Import slsls lifting.
 From simuliris.simplang Require Import proofmode tactics.
-From simuliris.simplang Require Import parallel_subst primitive_laws log_rel ctx.
-
-Section struct_val_rel.
-  Context `{!sheapGS Σ} `{!sheapInv Σ}.
-  Context (loc_rel : loc → loc → iProp Σ).
-
-  Fixpoint struct_val_rel (v_t v_s : val) {struct v_s} : iProp Σ :=
-    match v_t, v_s with
-    | LitV (LitLoc l_t), LitV (LitLoc l_s) =>
-        loc_rel l_t l_s
-    | LitV l_t, LitV l_s =>
-        ⌜l_t = l_s⌝
-    | PairV v1_t v2_t, PairV v1_s v2_s =>
-        struct_val_rel v1_t v1_s ∗ struct_val_rel v2_t v2_s
-    | InjLV v_t, InjLV v_s =>
-        struct_val_rel v_t v_s
-    | InjRV v_t, InjRV v_s =>
-        struct_val_rel v_t v_s
-    | _,_ => False
-    end.
-  Global Instance struct_val_rel_pers v_t v_s `{!∀ l_t l_s, Persistent (loc_rel l_t l_s)} :
-    Persistent (struct_val_rel v_t v_s).
-  Proof.
-    induction v_s as [[] | | | ] in v_t |-*; destruct v_t as [ [] | | | ]; apply _.
-  Qed.
-
-  Lemma struct_val_rel_pair_source v_t v_s1 v_s2 :
-    struct_val_rel v_t (v_s1, v_s2) -∗
-    ∃ v_t1 v_t2, ⌜v_t = PairV v_t1 v_t2⌝ ∗
-      struct_val_rel v_t1 v_s1 ∗
-      struct_val_rel v_t2 v_s2.
-  Proof.
-    simpl. iIntros "H". destruct v_t as [[] | v_t1 v_t2 | |]; simpl; try done.
-    iExists v_t1, v_t2. iDestruct "H" as "[$ $]". eauto.
-  Qed.
-  Lemma struct_val_rel_injl_source v_t v_s :
-    struct_val_rel v_t (InjLV v_s) -∗ ∃ v_t', ⌜v_t = InjLV v_t'⌝ ∗ struct_val_rel v_t' v_s.
-  Proof. simpl. destruct v_t as [[] | | |]; (try by iIntros "%Hp"); eauto. Qed.
-  Lemma struct_val_rel_injr_source v_t v_s :
-    struct_val_rel v_t (InjRV v_s) -∗ ∃ v_t', ⌜v_t = InjRV v_t'⌝ ∗ struct_val_rel v_t' v_s.
-  Proof. simpl. destruct v_t as [[] | | |]; (try by iIntros "%Hp"); eauto. Qed.
-
-
-  Lemma struct_val_rel_litfn_source v_t fn_s :
-    struct_val_rel v_t (LitV $ LitFn $ fn_s) -∗ ⌜v_t = LitV $ LitFn $ fn_s⌝.
-  Proof. simpl. destruct v_t as [[] | v_t1 v_t2 | |]; iIntros "%Hp"; inversion Hp; subst; done. Qed.
-  Lemma struct_val_rel_litint_source v_t n :
-    struct_val_rel v_t (LitV $ LitInt n) -∗ ⌜v_t = LitV $ LitInt $ n⌝.
-  Proof. simpl. destruct v_t as [[] | v_t1 v_t2 | |]; iIntros "%Hp"; inversion Hp; subst; done. Qed.
-  Lemma struct_val_rel_litbool_source v_t b:
-    struct_val_rel v_t (LitV $ LitBool b) -∗ ⌜v_t = LitV $ LitBool b⌝.
-  Proof. simpl. destruct v_t as [[] | v_t1 v_t2 | |]; iIntros "%Hp"; inversion Hp; subst; done. Qed.
-  Lemma struct_val_rel_litunit_source v_t :
-    struct_val_rel v_t (LitV $ LitUnit) -∗ ⌜v_t = LitV $ LitUnit⌝.
-  Proof. simpl. destruct v_t as [[] | v_t1 v_t2 | |]; iIntros "%Hp"; inversion Hp; subst; done. Qed.
-  Lemma struct_val_rel_litpoison_source v_t :
-    struct_val_rel v_t (LitV $ LitPoison) -∗ ⌜v_t = LitV $ LitPoison⌝.
-  Proof. simpl. destruct v_t as [[] | v_t1 v_t2 | |]; iIntros "%Hp"; inversion Hp; subst; done. Qed.
-  Lemma struct_val_rel_loc_source v_t l_s :
-    struct_val_rel v_t (LitV $ LitLoc l_s) -∗
-    ∃ l_t, ⌜v_t = LitV $ LitLoc l_t⌝ ∗ loc_rel l_t l_s.
-  Proof.
-    destruct v_t as [[ | | | | l_t | ] | | | ]; simpl;
-        first [iIntros "%Ht"; congruence | iIntros "Ht"; eauto].
-  Qed.
-
-  Lemma struct_val_rel_pair_target v_s v_t1 v_t2 :
-    struct_val_rel (v_t1, v_t2) v_s -∗
-    ∃ v_s1 v_s2, ⌜v_s = PairV v_s1 v_s2⌝ ∗
-      struct_val_rel v_t1 v_s1 ∗
-      struct_val_rel v_t2 v_s2.
-  Proof.
-    simpl. iIntros "H". destruct v_s as [[] | v_s1 v_s2 | |]; simpl; try done.
-    iExists v_s1, v_s2. iDestruct "H" as "[$ $]". eauto.
-  Qed.
-  Lemma struct_val_rel_injl_target v_t v_s :
-    struct_val_rel (InjLV v_t) v_s -∗ ∃ v_s', ⌜v_s = InjLV v_s'⌝ ∗ struct_val_rel v_t v_s'.
-  Proof. simpl. destruct v_s as [[] | | |]; (try by iIntros "%Hp"); eauto. Qed.
-  Lemma struct_val_rel_injr_target v_t v_s :
-    struct_val_rel (InjRV v_t) v_s -∗ ∃ v_s', ⌜v_s = InjRV v_s'⌝ ∗ struct_val_rel v_t v_s'.
-  Proof. simpl. destruct v_s as [[] | | |]; (try by iIntros "%Hp"); eauto. Qed.
-  Lemma struct_val_rel_litfn_target v_s fn_t :
-    struct_val_rel (LitV $ LitFn $ fn_t) v_s -∗ ⌜v_s = LitV $ LitFn $ fn_t⌝.
-  Proof. simpl. destruct v_s as [[] | v_s1 v_s2 | |]; iIntros "%Hp"; inversion Hp; subst; done. Qed.
-  Lemma struct_val_rel_litint_target v_s n :
-    struct_val_rel (LitV $ LitInt n) v_s -∗ ⌜v_s = LitV $ LitInt $ n⌝.
-  Proof. simpl. destruct v_s as [[] | | |]; iIntros "%Hp"; inversion Hp; subst; done. Qed.
-  Lemma struct_val_rel_litbool_target v_s b:
-    struct_val_rel (LitV $ LitBool b) v_s -∗ ⌜v_s = LitV $ LitBool b⌝.
-  Proof. simpl. destruct v_s as [[] | | |]; iIntros "%Hp"; inversion Hp; subst; done. Qed.
-  Lemma struct_val_rel_litunit_target v_s :
-    struct_val_rel (LitV $ LitUnit) v_s -∗ ⌜v_s = LitV $ LitUnit⌝.
-  Proof. simpl. destruct v_s as [[] | | |]; iIntros "%Hp"; inversion Hp; subst; done. Qed.
-  Lemma struct_val_rel_litpoison_target v_s :
-    struct_val_rel (LitV $ LitPoison) v_s -∗ ⌜v_s = LitV $ LitPoison⌝.
-  Proof. simpl. destruct v_s as [[] | | |]; iIntros "%Hp"; inversion Hp; subst; done. Qed.
-  Lemma struct_val_rel_loc_target v_s l_t :
-    struct_val_rel (LitV $ LitLoc l_t) v_s -∗
-    ∃ l_s, ⌜v_s = LitV $ LitLoc l_s⌝ ∗ loc_rel l_t l_s.
-  Proof.
-    destruct v_s as [[ | | | | l_s | ] | | | ]; simpl;
-        first [iIntros "%Hs"; congruence | iIntros "Hs"; eauto].
-  Qed.
-
-End struct_val_rel.
-Tactic Notation "val_discr_source" constr(H) :=
-  first [iPoseProof (struct_val_rel_litint_source with H) as "->" |
-         iPoseProof (struct_val_rel_litbool_source with H) as "->" |
-         iPoseProof (struct_val_rel_litfn_source with H) as "->" |
-         iPoseProof (struct_val_rel_litunit_source with H) as "->" |
-         iPoseProof (struct_val_rel_litpoison_source with H) as "->" |
-         idtac].
-Tactic Notation "val_discr_target" constr(H) :=
-  first [iPoseProof (struct_val_rel_litint_target with H) as "->" |
-         iPoseProof (struct_val_rel_litbool_target with H) as "->" |
-         iPoseProof (struct_val_rel_litfn_target with H) as "->" |
-         iPoseProof (struct_val_rel_litunit_target with H) as "->" |
-         iPoseProof (struct_val_rel_litpoison_target with H) as "->" |
-         idtac].
+From simuliris.simplang Require Import parallel_subst primitive_laws gen_val_rel gen_log_rel wf.
 
 Section log_rel.
   Context `{!sheapGS Σ} `{!sheapInv Σ}.
   Context (loc_rel : loc → loc → iProp Σ) `{!∀ l_t l_s, Persistent (loc_rel l_t l_s)}.
   Context (thread_own : thread_id → iProp Σ).
-  Notation val_rel := (struct_val_rel loc_rel) (only parsing).
-  Notation log_rel := (log_rel val_rel thread_own) (only parsing).
+  Let val_rel := (gen_val_rel loc_rel).
+  Let log_rel := (gen_log_rel loc_rel thread_own).
 
   Lemma val_wf_sound v : val_wf v → ⊢ val_rel v v.
   Proof.
@@ -140,24 +22,24 @@ Section log_rel.
     destruct to_fname; [destruct to_val | ]; done.
   Qed.
 
-  Lemma struct_val_rel_val_is_unboxed v_t v_s : val_rel v_t v_s -∗ ⌜val_is_unboxed v_t ↔ val_is_unboxed v_s⌝.
+  Lemma gen_val_rel_val_is_unboxed v_t v_s : val_rel v_t v_s -∗ ⌜val_is_unboxed v_t ↔ val_is_unboxed v_s⌝.
   Proof.
     iIntros "Hv".
     destruct v_s as [[] | | | ]; val_discr_source "Hv"; [ done .. | |done | | |].
-    - by iPoseProof (struct_val_rel_loc_source with "Hv") as (?) "(-> & _)".
-    - by iPoseProof (struct_val_rel_pair_source with "Hv") as (??) "(-> & Hv1 & Hv2)".
-    - iPoseProof (struct_val_rel_injl_source with "Hv") as (?) "(-> & Hv)".
+    - by iPoseProof (gen_val_rel_loc_source with "Hv") as (?) "(-> & _)".
+    - by iPoseProof (gen_val_rel_pair_source with "Hv") as (??) "(-> & Hv1 & Hv2)".
+    - iPoseProof (gen_val_rel_injl_source with "Hv") as (?) "(-> & Hv)".
       destruct v_s as [[] | | | ]; val_discr_source "Hv"; [done.. | | done | | |].
-      + by iPoseProof (struct_val_rel_loc_source with "Hv") as (?) "(-> & _)".
-      + by iPoseProof (struct_val_rel_pair_source with "Hv") as (??) "(-> & Hv1 & Hv2)".
-      + by iPoseProof (struct_val_rel_injl_source with "Hv") as (?) "(-> & Hv)".
-      + by iPoseProof (struct_val_rel_injr_source with "Hv") as (?) "(-> & Hv)".
-    - iPoseProof (struct_val_rel_injr_source with "Hv") as (?) "(-> & Hv)".
+      + by iPoseProof (gen_val_rel_loc_source with "Hv") as (?) "(-> & _)".
+      + by iPoseProof (gen_val_rel_pair_source with "Hv") as (??) "(-> & Hv1 & Hv2)".
+      + by iPoseProof (gen_val_rel_injl_source with "Hv") as (?) "(-> & Hv)".
+      + by iPoseProof (gen_val_rel_injr_source with "Hv") as (?) "(-> & Hv)".
+    - iPoseProof (gen_val_rel_injr_source with "Hv") as (?) "(-> & Hv)".
       destruct v_s as [[] | | | ]; val_discr_source "Hv"; [done.. | | done | | |].
-      + by iPoseProof (struct_val_rel_loc_source with "Hv") as (?) "(-> & _)".
-      + by iPoseProof (struct_val_rel_pair_source with "Hv") as (??) "(-> & Hv1 & Hv2)".
-      + by iPoseProof (struct_val_rel_injl_source with "Hv") as (?) "(-> & Hv)".
-      + by iPoseProof (struct_val_rel_injr_source with "Hv") as (?) "(-> & Hv)".
+      + by iPoseProof (gen_val_rel_loc_source with "Hv") as (?) "(-> & _)".
+      + by iPoseProof (gen_val_rel_pair_source with "Hv") as (??) "(-> & Hv1 & Hv2)".
+      + by iPoseProof (gen_val_rel_injl_source with "Hv") as (?) "(-> & Hv)".
+      + by iPoseProof (gen_val_rel_injr_source with "Hv") as (?) "(-> & Hv)".
   Qed.
 
   Local Tactic Notation "smart_sim_bind" uconstr(ctx_t) uconstr(ctx_s) uconstr(Hp) :=
@@ -214,9 +96,12 @@ Section log_rel.
   Qed.
 
   Lemma log_rel_binop e1_t e1_s e2_t e2_s o :
+    loc_rel_func_law loc_rel →
+    loc_rel_inj_law loc_rel →
+    loc_rel_offset_law loc_rel →
     log_rel e1_t e1_s -∗ log_rel e2_t e2_s -∗ log_rel (BinOp o e1_t e2_t) (BinOp o e1_s e2_s).
   Proof.
-    iIntros "#IH1 #IH2" (? xs) "!# #Hs Ht"; simpl.
+    iIntros (Hfunc Hinj Hshift). iIntros "#IH1 #IH2" (? xs) "!# #Hs Ht"; simpl.
     smart_sim_bind (subst_map _ e2_t) (subst_map _ e2_s) "(IH2 [] Ht)".
     { iApply (subst_map_rel_weaken with "[$]"). set_solver. }
     iIntros (v_t2 v_s2) "[Ht Hv2]".
@@ -225,22 +110,16 @@ Section log_rel.
     iIntros (v_t1 v_s1) "[Ht Hv1]".
     destruct o; sim_pures; discr_source; val_discr_source "Hv1"; val_discr_source "Hv2"; sim_pures; [sim_val; by iFrame .. | | ].
     - iAssert (⌜vals_compare_safe v_t1 v_t2⌝)%I as "%".
-      { iPoseProof (struct_val_rel_val_is_unboxed with "Hv1") as "%Hv1".
-        iPoseProof (struct_val_rel_val_is_unboxed with "Hv2") as "%Hv2".
+      { iPoseProof (gen_val_rel_val_is_unboxed with "Hv1") as "%Hv1".
+        iPoseProof (gen_val_rel_val_is_unboxed with "Hv2") as "%Hv2".
         iPureIntro. by rewrite /vals_compare_safe Hv1 Hv2.
       }
-      case_bool_decide; subst; sim_pures; sim_val; iFrame.
-      * admit.
-        (* iPoseProof (struct_val_rel_inj with "Hv1 Hv2") as "->". *)
-        (* sim_pures; sim_val. case_bool_decide; done. *)
-      * admit.
-        (* sim_pures; sim_val. case_bool_decide; subst; last done. *)
-        (* by iPoseProof (val_rel_func with "Hv1 Hv2") as "->". *)
-    - iPoseProof (struct_val_rel_loc_source with "Hv1") as (l_t) "(-> & Hl)".
-      sim_pures. sim_val. iModIntro; cbn.
-      admit.
-      (* by iApply heap_bij_loc_shift. *)
-  Admitted.
+      sim_pures; sim_val. iFrame. case_bool_decide; subst.
+      * iDestruct (gen_val_rel_func with "Hv1 Hv2") as %->; [done|]. by case_bool_decide.
+      * case_bool_decide; [|done]; subst. by iDestruct (gen_val_rel_inj with "Hv1 Hv2") as %?.
+    - iPoseProof (gen_val_rel_loc_source with "Hv1") as (l_t) "(-> & Hl)".
+      sim_pures. sim_val. iModIntro; simpl. iFrame. by iApply Hshift.
+  Qed.
 
   Lemma log_rel_if e1_t e1_s e2_t e2_s e3_t e3_s :
     log_rel e1_t e1_s -∗
@@ -298,7 +177,7 @@ Section log_rel.
     { iApply (subst_map_rel_weaken with "[$]"). set_solver. }
     iIntros (v_t v_s) "[Ht Hv]".
     discr_source.
-    iPoseProof (struct_val_rel_pair_source with "Hv") as (??) "(-> & ? & ?)"; sim_pures; sim_val; by iFrame.
+    iPoseProof (gen_val_rel_pair_source with "Hv") as (??) "(-> & ? & ?)"; sim_pures; sim_val; by iFrame.
   Qed.
   Lemma log_rel_snd e_t e_s :
     log_rel e_t e_s -∗ log_rel (Snd e_t) (Snd e_s).
@@ -308,7 +187,7 @@ Section log_rel.
     { iApply (subst_map_rel_weaken with "[$]"). set_solver. }
     iIntros (v_t v_s) "[Ht Hv]".
     discr_source.
-    iPoseProof (struct_val_rel_pair_source with "Hv") as (??) "(-> & ? & ?)"; sim_pures; sim_val; by iFrame.
+    iPoseProof (gen_val_rel_pair_source with "Hv") as (??) "(-> & ? & ?)"; sim_pures; sim_val; by iFrame.
   Qed.
 
   Lemma log_rel_injl e_t e_s :
@@ -339,7 +218,7 @@ Section log_rel.
     { iApply (subst_map_rel_weaken with "[$]"). set_solver. }
     iIntros (v_t v_s) "[Ht #Hv]".
     discr_source.
-    + iPoseProof (struct_val_rel_injl_source with "Hv") as (v_t') "(-> & ?)". sim_pures.
+    + iPoseProof (gen_val_rel_injl_source with "Hv") as (v_t') "(-> & ?)". sim_pures.
       rewrite !subst'_subst_map.
       rewrite -(binder_insert_fmap fst (v_t', x)).
       rewrite -(binder_insert_fmap snd (v_t', x)).
@@ -349,7 +228,7 @@ Section log_rel.
       destruct x1 as [|x1]; first set_solver.
       apply elem_of_subseteq=>x'.
       destruct (decide (x1 = x')) as [<-|Hne]; set_solver.
-    + iPoseProof (struct_val_rel_injr_source with "Hv") as (v_t') "(-> & ?)". sim_pures.
+    + iPoseProof (gen_val_rel_injr_source with "Hv") as (v_t') "(-> & ?)". sim_pures.
       rewrite !subst'_subst_map.
       rewrite -(binder_insert_fmap fst (v_t', x)).
       rewrite -(binder_insert_fmap snd (v_t', x)).
@@ -407,8 +286,8 @@ Section log_rel.
     smart_sim_bind (subst_map _ _) (subst_map _ _) "(IH1 [] Ht)".
     { iApply (subst_map_rel_weaken with "[$]"). set_solver. }
     iIntros (v_t' v_s') "[Ht Hv']".
-    discr_source. iPoseProof (struct_val_rel_loc_source with "Hv") as (l_t) "(-> & Hrel)".
-    iPoseProof (struct_val_rel_litint_source with "Hv'") as "->".
+    discr_source. iPoseProof (gen_val_rel_loc_source with "Hv") as (l_t) "(-> & Hrel)".
+    iPoseProof (gen_val_rel_litint_source with "Hv'") as "->".
     iApply (Hfree with "Ht Hrel"); [done|].
     iIntros "Ht". sim_val. by iFrame.
   Qed.
@@ -424,7 +303,7 @@ Section log_rel.
     smart_sim_bind (subst_map _ _) (subst_map _ _) "(IH [] Ht)".
     { iApply (subst_map_rel_weaken with "[$]"). set_solver. }
     iIntros (v_t v_s) "[Ht Hv]". discr_source.
-    iPoseProof (struct_val_rel_loc_source with "Hv") as (l_t) "(-> & Hrel)".
+    iPoseProof (gen_val_rel_loc_source with "Hv") as (l_t) "(-> & Hrel)".
     iApply (Hload with "Ht Hrel").
     iIntros (v_t v_s) "Ht Hrel". sim_val; by iFrame.
   Qed.
@@ -443,7 +322,7 @@ Section log_rel.
     smart_sim_bind (subst_map _ _) (subst_map _ _) "(IH1 [] Ht)".
     { iApply (subst_map_rel_weaken with "[$]"). set_solver. }
     iIntros (v_t' v_s') "[Ht Hv']".
-    discr_source. iPoseProof (struct_val_rel_loc_source with "Hv'") as (l_t) "(-> & Hrel)".
+    discr_source. iPoseProof (gen_val_rel_loc_source with "Hv'") as (l_t) "(-> & Hrel)".
     iApply (Hstore with "Ht Hrel Hv").
     iIntros "Ht". sim_val; by iFrame.
   Qed.
@@ -451,35 +330,4 @@ Section log_rel.
   Lemma log_rel_val v_t v_s :
     val_rel v_t v_s -∗ log_rel (Val v_t) (Val v_s).
   Proof. iIntros "#Hv" (? xs) "!# #Hs Ht"; simpl. sim_val; by iFrame. Qed.
-
-  Definition pure_expr_wf (e : expr) : Prop :=
-    match e with
-    | Val v => val_wf v
-    | Var _ | Let _ _ _ | UnOp _ _ | BinOp _ _ _ | If _ _ _ | While _ _
-    | Pair _ _ | Fst _ | Snd _ | InjL _ | InjR _ | Match _ _ _ _ _ => True
-    | _ => False
-    end.
-
-  Theorem pure_expr_wf_sound : log_rel_exprs pure_expr_wf val_rel thread_own.
-  Proof.
-    intros e_t e_s Hwf Hs. iIntros "IH".
-    destruct e_t; simpl in Hs; destruct e_s => //=; simpl in Hs; simplify_eq.
-    all: try iDestruct "IH" as "[IH IH1]".
-    all: try iDestruct "IH1" as "[IH1 IH2]".
-    all: try iDestruct "IH2" as "[IH2 IH3]".
-    - (* Val *) iApply log_rel_val. by iApply val_wf_sound.
-    - (* Var *) by iApply log_rel_var.
-    - (* Let *) by iApply (log_rel_let with "IH IH1").
-    - (* UnOp *) by iApply (log_rel_unop with "IH").
-    - (* BinOp *) by iApply (log_rel_binop with "IH IH1").
-    - (* If *) by iApply (log_rel_if with "IH IH1 IH2").
-    - (* While *) by iApply (log_rel_while with "IH IH1").
-    - (* Pairs *) by iApply (log_rel_pair with "IH IH1").
-    - (* Fst *) by iApply (log_rel_fst with "IH").
-    - (* Snd *) by iApply (log_rel_snd with "IH").
-    - (* InjL *) by iApply (log_rel_injl with "IH").
-    - (* InjR *) by iApply (log_rel_injr with "IH").
-    - (* Match *) destruct_and!; simplify_eq.
-      by iApply (log_rel_match with "IH IH1 IH2").
-  Qed.
 End log_rel.
