theories/simplang/base.v
@@ -1,0 +1,56 @@
+From iris.proofmode Require Import tactics.
+
+(* TODO: upstream the following definitions *)
+Lemma take_lookup_Some {A} n k (l : list A) x:
+  take n l !! k = Some x ↔ l !! k = Some x ∧ k < n.
+Proof.
+  split.
+  - destruct (decide (k < n)).
+    + rewrite lookup_take; naive_solver.
+    + rewrite lookup_take_ge //. lia.
+  - move => [??]. by rewrite lookup_take.
+Qed.
+
+Lemma map_seq_insert_0 {A} (ls : list A) i x:
+  i < length ls →
+  <[i:=x]> (map_seq (M :=gmap _ _) 0 ls) = map_seq 0 (<[i:=x]>ls).
+Proof.
+  move => ?. apply: map_eq => j. rewrite lookup_map_seq_0.
+  destruct (decide (i = j)); simplify_map_eq.
+  - by rewrite list_lookup_insert.
+  - by rewrite lookup_map_seq_0 list_lookup_insert_ne.
+Qed.
+
+Lemma big_sepL2_exist {PROP : bi} {A B C} (l1 : list A) (l2 : list B) (Φ : _ → _ → _ → _ → PROP) `{!BiAffine PROP} :
+  ([∗ list] i↦x1;x2∈l1;l2, ∃ x : C, Φ i x1 x2 x) -∗
+   ∃ xs : list C, ⌜length xs = length l1⌝ ∗ ([∗ list] i↦x1;x2∈l1;l2, ∃ x : C, ⌜xs !! i = Some x⌝ ∗ Φ i x1 x2 x).
+Proof.
+  iIntros "Hl".
+  iInduction (l1) as [|? l1] "IH" forall (l2 Φ).
+  { iDestruct (big_sepL2_nil_inv_l with "Hl") as %->. iExists []. by iSplit. }
+  iDestruct (big_sepL2_cons_inv_l with "Hl") as (x2 l2' ->) "[[%x ?] Hl]".
+  iDestruct ("IH" with "Hl") as (xs) "[%Heq ?]".
+  iExists (x::xs) => /=. iSplit; [by rewrite /= Heq|]. iFrame.
+  iExists _. by iFrame.
+Qed.
+Lemma big_sepL2_to_sepL_r {PROP : bi} {A B} (l1 : list A) (l2 : list B) (Φ : _ → _ → _ → PROP) `{!BiAffine PROP}:
+  length l1 = length l2 →
+  ([∗ list] i↦x1;x2∈l1;l2, Φ i x1 x2) ⊣⊢
+  ([∗ list] i↦x2∈l2, ∃ x1, ⌜l1 !! i = Some x1⌝ ∗  Φ i x1 x2).
+Proof.
+  elim: l1 l2 Φ. { by case. }
+  move => x l1 IH [//|y l2] Φ /= [?]. rewrite IH //. f_equiv.
+  iSplit; first by eauto with iFrame. iIntros "[%x1 [% ?]]"; by simplify_eq.
+Qed.
+
+Definition exists_dec_unique {A} (x : A) (P : _ → Prop) : (∀ y, P y → P x) → Decision (P x) → Decision (∃ y, P y).
+Proof.
+  intros Hx Hdec.
+  refine (cast_if (decide (P x))).
+  - abstract by eexists _.
+  - abstract naive_solver.
+Defined.
+
+Lemma forall_equiv_dec {X} (P Q : X → Prop) (HPQ : Decision (∀ x, P x → Q x)) (HQP : Decision (∀ x, Q x → P x)) :
+  Decision (∀ x, P x ↔ Q x).
+Proof. destruct HPQ as [HPQ | HPQ]; destruct HQP as [HQP | HQP]; [left; naive_solver | right; naive_solver..]. Qed.
