theories/simplang/examples/sum.v
@@ -4,12 +4,14 @@ Import bi.
 From iris.proofmode Require Import tactics.
 From simuliris.simulation Require Import slsls lifting.
 
-(** This file defines a simple value relation for encoding sums using pairs and shows a simple example program.
-  This example is not fully worked out (the relation does not have support for heap operations).*)
+(** This file defines a simple value relation for encoding sums using
+  pairs and shows a simple example program. This example is not fully
+  worked out (the relation does not have support for heap operations),
+  and there is no reflexivity or adequacy theorem proven.*)
 
 
 Section fix_bi.
-Context `{sheapGS Σ} (π : thread_id).
+Context `{sheapGS Σ}.
 Inductive val_rel_pure : val → val → Prop :=
   | val_rel_lit l : val_rel_pure (LitV l) (LitV l)
   | val_rel_injL v1 v2 : val_rel_pure v1 v2 → val_rel_pure ((#1, v1)%V) (InjLV v2)
@@ -25,7 +27,7 @@ Program Instance : sheapInv Σ := {|
   sheap_ext_rel _ := val_rel;
  |}.
 Next Obligation. done. Qed.
-Global Instance : sheapInvSupportsAll.
+Global Instance : sheapInvStateIndependent.
 Proof. done. Qed.
 
 (* Sums are encoded as injL x -> (1, x); injR x -> (2, x); the tag encodes the constructor.  *)
@@ -36,8 +38,6 @@ Definition inj2_enc : ectx := (λ: "x", (#2, "x"))%E.
 Definition diverge : ectx := (λ: "x", Call "diverge" "x")%E.
 
 (** the value relation determining which values can be passed to a function *)
-
-Local Notation "et '⪯' es {{ Φ }}" := (et ⪯{π} es {{Φ}})%I (at level 40, Φ at level 200) : bi_scope.
 
 Definition mul2_source :=
   (λ: "x",
@@ -56,9 +56,9 @@ Definition mul2_target :=
 Definition source_prog : gmap string ectx := {[ "inj1_enc" := inj1_enc; "diverge" := diverge; "mul2" := mul2_source ]}.
 Definition target_prog : gmap string ectx := {[ "diverge" := diverge; "mul2" := mul2_target]}.
 
-Lemma mul2_sim:
+Lemma mul2_sim π:
   ⊢ ∀ v_t v_s, val_rel v_t v_s -∗
-    fill mul2_target (of_val v_t) ⪯ fill mul2_source (of_val v_s) {{ λ v_t' v_s', val_rel v_t' v_s' }}.
+    fill mul2_target (of_val v_t) ⪯{π} fill mul2_source (of_val v_s) {{ λ v_t' v_s', val_rel v_t' v_s' }}.
 Proof.
   iIntros (?? Hval). rewrite /mul2_target /mul2_source.
   sim_pures.
@@ -80,11 +80,11 @@ Qed.
 Definition source_client := (λ: "x", Call (##"mul2") (InjL "x"))%E.
 Definition target_client := (λ: "x", Call (## "mul2") (Call (##"inj1_enc") "x"))%E.
 
-Lemma client_sim (n : Z) :
+Lemma client_sim (n : Z) π :
   "target_client" @t target_client -∗
   "source_client" @s source_client -∗
   "inj1_enc" @t inj1_enc -∗
-  Call (##"target_client") #n ⪯ Call (##"source_client") #n {{ λ v_t v_s, val_rel v_t v_s }}.
+  Call (##"target_client") #n ⪯{π} Call (##"source_client") #n {{ λ v_t v_s, val_rel v_t v_s }}.
 Proof.
   iIntros "Htarget Hsource Hinj1_t".
   target_call. target_call. source_call. sim_pures.
