theories/simplang/simple_inv/examples/reorder_malloc.v
@@ -1,12 +1,12 @@
-From simuliris.simplang Require Import lang notation tactics class_instances log_rel.
+From simuliris.simplang Require Import lang notation tactics class_instances gen_log_rel.
 From iris.proofmode Require Import tactics.
 From simuliris.simulation Require Import slsls lifting.
-From simuliris.simplang.simple_inv Require Import simple_inv.
+From simuliris.simplang.simple_inv Require Import inv.
 
 (** * Simple example for re-ordering two allocs and then passing the related locations to an external function. *)
 
 Section reorder.
-  Context `{heapbijG Σ}.
+  Context `{!simpleGS Σ}.
 
   Definition alloc2_and_cont : expr :=
     let: "l1" := Alloc "v1" in
@@ -19,7 +19,7 @@ Section reorder.
     Call "cont" ("l1", "l2").
 
   Lemma alloc2_reorder :
-    ⊢ log_rel val_rel (const True%I) alloc2_and_cont alloc2_and_cont'.
+    ⊢ log_rel alloc2_and_cont alloc2_and_cont'.
   Proof.
     log_rel.
     iIntros "%cont_t %cont_s #Hcont %v1_t %v1_s #Hv1 %v2_t %v2_s #Hv2 !# %π _".
