theories/simplang/wf.v
@@ -1,0 +1,99 @@
+From simuliris.simplang Require Import lang.
+
+(** * "Well-formed" values and expressions.
+These definitions basically form our type system. Their main job is to
+exclude programs that contain literal locations.  *)
+
+Fixpoint val_wf (v : val) : Prop :=
+  match v with
+  | LitV (LitLoc l) => False (* no literal locations allowed *)
+  | LitV _ => True
+  | PairV v1 v2 => val_wf v1 ∧ val_wf v2
+  | InjLV v => val_wf v
+  | InjRV v => val_wf v
+  end.
+
+(** This defines a re-usable notion of well-formedness for expressions,
+evaluation contexts, and general contexts that can be tweaked by
+adjusting [expr_head_wf]. *)
+Section expr_wf.
+
+  Context (expr_head_wf : expr_head → Prop).
+
+  (** Lift [expr_head_wf] to expressions. *)
+  Fixpoint gen_expr_wf (e : expr) : Prop :=
+    expr_head_wf (expr_split_head e).1 ∧
+    match e with
+    | Val v => True (** [val_wf v] should be part of [expr_head_wf (Val
+      v)] because [log_rel_structural] only provides [expr_head_wf]. *)
+    | Var x => True
+    | Let b e1 e2 => gen_expr_wf e1 ∧ gen_expr_wf e2
+    | Call e1 e2 => gen_expr_wf e1 ∧ gen_expr_wf e2
+    | UnOp op e => gen_expr_wf e
+    | BinOp op e1 e2 => gen_expr_wf e1 ∧ gen_expr_wf e2
+    | If e1 e2 e3 => gen_expr_wf e1 ∧ gen_expr_wf e2 ∧ gen_expr_wf e3
+    | While e1 e2 => gen_expr_wf e1 ∧ gen_expr_wf e2
+    | Pair e1 e2 => gen_expr_wf e1 ∧ gen_expr_wf e2
+    | Fst e => gen_expr_wf e
+    | Snd e => gen_expr_wf e
+    | InjL e => gen_expr_wf e
+    | InjR e => gen_expr_wf e
+    | Match e x1 e1 x2 e2 => gen_expr_wf e ∧ gen_expr_wf e1 ∧ gen_expr_wf e2
+    | Fork e => gen_expr_wf e
+    | AllocN e1 e2 => gen_expr_wf e1 ∧ gen_expr_wf e2
+    | FreeN e1 e2 => gen_expr_wf e1 ∧ gen_expr_wf e2
+    | Load o e => gen_expr_wf e
+    | Store o e1 e2 => gen_expr_wf e1 ∧ gen_expr_wf e2
+    | CmpXchg e1 e2 e3 => gen_expr_wf e1 ∧ gen_expr_wf e2 ∧ gen_expr_wf e3
+    | FAA e1 e2 => gen_expr_wf e1 ∧ gen_expr_wf e2
+    end.
+
+  (** Lift [expr_head_wf] to evaluation contexts. *)
+  Definition gen_ectxi_wf (Ki : ectx_item) : Prop :=
+    let head := ectxi_split_head Ki in
+    expr_head_wf head.1 ∧ Forall gen_expr_wf head.2.
+  Definition gen_ectx_wf : ectx → Prop := Forall gen_ectxi_wf.
+
+  Lemma gen_ectx_wf_cons C Ci :
+    gen_ectx_wf (Ci :: C) ↔ gen_ectxi_wf Ci ∧ gen_ectx_wf C.
+  Proof. rewrite /gen_ectx_wf Forall_cons //. Qed.
+  Lemma gen_ectx_wf_app C1 C2 :
+    gen_ectx_wf (C1 ++ C2) ↔ gen_ectx_wf C1 ∧ gen_ectx_wf C2.
+  Proof. apply Forall_app. Qed.
+  Lemma gen_ectx_wf_snoc C Ci :
+    gen_ectx_wf (C ++ [Ci]) ↔ gen_ectx_wf C ∧ gen_ectxi_wf Ci.
+  Proof. rewrite gen_ectx_wf_app /gen_ectx_wf Forall_singleton //. Qed.
+
+  (** Lift [expr_head_wf] to contexts. *)
+  Definition gen_ctxi_wf (Ci : ctx_item) : Prop :=
+    let head := ctxi_split_head Ci in
+    expr_head_wf head.1 ∧ Forall gen_expr_wf head.2.
+  Definition gen_ctx_wf : ctx → Prop := Forall gen_ctxi_wf.
+
+  Lemma gen_ctx_wf_cons C Ci :
+    gen_ctx_wf (Ci :: C) ↔ gen_ctxi_wf Ci ∧ gen_ctx_wf C.
+  Proof. rewrite /gen_ctx_wf Forall_cons //. Qed.
+  Lemma gen_ctx_wf_app C1 C2 :
+    gen_ctx_wf (C1 ++ C2) ↔ gen_ctx_wf C1 ∧ gen_ctx_wf C2.
+  Proof. apply Forall_app. Qed.
+  Lemma gen_ctx_wf_snoc C Ci :
+    gen_ctx_wf (C ++ [Ci]) ↔ gen_ctx_wf C ∧ gen_ctxi_wf Ci.
+  Proof. rewrite gen_ctx_wf_app /gen_ctx_wf Forall_singleton //. Qed.
+
+  Lemma expr_gen_egen_ctx_wf_fill e Ks :
+    gen_expr_wf (fill Ks e) ↔ gen_expr_wf e ∧ gen_ectx_wf Ks.
+  Proof.
+    elim: Ks e => /=.
+    { unfold gen_ectx_wf. naive_solver. }
+    move => K Ks IH e. rewrite IH gen_ectx_wf_cons /gen_ectxi_wf.
+    destruct K => /=; rewrite ?Forall_cons ?Forall_nil /=; naive_solver.
+  Qed.
+  Lemma expr_gen_ctx_wf_fill e Cs :
+    gen_expr_wf (fill_ctx Cs e) ↔ gen_expr_wf e ∧ gen_ctx_wf Cs.
+  Proof.
+    elim: Cs e => /=.
+    { unfold gen_ctx_wf. naive_solver. }
+    move => C Cs IH e. rewrite IH gen_ctx_wf_cons /gen_ctxi_wf.
+    destruct C => /=; rewrite ?Forall_cons ?Forall_nil /=; naive_solver.
+  Qed.
+End expr_wf.
